Prove that moves preserve the well-formed property

TicTacToe/Basic.lean
@@ -1,3 +1,80 @@
+-- Helper theorems
+
+def vector_cons : α → Vector α n → Vector α (Nat.succ n)
+  | a, ⟨v, h⟩ =>
+    have hSize : (a :: v.toList).toArray.size = Nat.succ n := by grind
+    Vector.mk (n := Nat.succ n) (List.toArray (a :: Array.toList v)) hSize
+
+theorem vector_cons_equivalence {α} {xs : Vector α (Nat.succ n)} : xs = vector_cons xs.head xs.tail := by
+  apply Vector.ext
+  intro i
+  induction i with
+  | zero => simp [vector_cons, Vector.head]
+  | succ i ih =>
+    intro hIndexWithinBounds
+    unfold vector_cons
+    simp
+
+theorem vector_cons_set {xs : Vector α n} {i : Fin (Nat.succ n)} : (vector_cons x xs).set i a = if hEq : i.val == 0 then vector_cons a xs else let n' := i.pred (by simp at hEq; simp [hEq]); vector_cons x (xs.set n' a) := by
+  by_cases h : (i = 0)
+  . simp [h, vector_cons, Vector.set]
+  . simp [h, vector_cons, Vector.set]
+    let i' := Fin.pred i h
+    rw [List.set.eq_def]
+    cases i using Fin.cases with
+    | zero => simp; grind
+    | succ => simp
+
+theorem vector_cons_get {xs : Vector α n} {i : Fin (Nat.succ n)} : (vector_cons x xs).get i = if hEq : i.val == 0 then x else let n' := i.pred (by simp at hEq; simp [hEq]); xs.get n' := by
+  by_cases h : (i = 0)
+  . simp [h, vector_cons, Vector.get]
+  . simp [h, vector_cons, Vector.get]
+    let i' := Fin.pred i h
+    simp only [GetElem.getElem]
+    rw [List.get.eq_def]
+    simp
+    cases i using Fin.cases with
+    | zero => simp; grind
+    | succ => simp [Vector.get]
+
+theorem vectorSetGetUnchanged
+    {α : Type} {n : Nat} (xs : Vector α n) (value : α)
+    (iSet iGet : Fin n) (hDistinct : iSet ≠ iGet) :
+    (Vector.set xs iSet value).get iGet = xs.get iGet := by
+  -- Revert these values, because their types vary per case
+  revert xs iSet iGet
+  cases n with
+  | zero =>
+      intro _ iSet
+      exact Fin.elim0 iSet
+  | succ n' =>
+      -- Going into the structure of the indices lets Lean see that they target different places
+      -- in the array
+      intro xs iSet iGet hDistinct
+      cases iSet using Fin.cases with
+      | zero =>
+          cases iGet using Fin.cases with
+          | zero => contradiction -- iSet = iGet = zero
+          | succ iGet' => simp [Vector.set, Vector.get] -- iGet > iSet
+      | succ iSet' =>
+          cases iGet using Fin.cases with
+          | zero => simp [Vector.set, Vector.get] -- iGet < iSet
+          | succ iGet' =>
+              -- iGet != iSet, but Lean can't see it because they are both `succ`, so we'll use
+              -- induction
+
+              rw [
+                vector_cons_equivalence (xs := xs),
+                vector_cons_set (x := xs.head) (xs := xs.tail) (i := iSet'.succ) (a := value),
+                vector_cons_get (x := xs.head) (xs := xs.tail) (i := iGet'.succ),
+              ]
+
+              have hDistinct' : iSet' ≠ iGet' := by grind
+              let ih := vectorSetGetUnchanged xs.tail value iSet' iGet' hDistinct'
+              by_cases h : (↑iSet'.succ == 0)
+              . simpa [h]
+              . simpa [h]
+
 -- Tic-tac-toe game
 
 inductive Player where
@@ -9,6 +86,9 @@ inductive Cell where
   | Empty : Cell
   | Occupied : Player → Cell
 deriving Repr, DecidableEq
+
+theorem cellNeqEmptyOccupied {player} : (Cell.Empty == Cell.Occupied player) = false := by
+  grind
 
 def Board := Vector Cell 9
 def Position := Fin 9
@@ -29,15 +109,24 @@ def emptyBoard : Board :=
 def initialGameState : TicTacToeState :=
   { board := emptyBoard, status := GameStatus.InProgress Player.X }
 
-def isEmptyPosition (board : Board) (pos : Position) : Bool :=
-  match board.get pos with
-  | Cell.Empty => true
-  | Cell.Occupied _ => false
+def isEmptyPosition (board : Board) (pos : Position) : Bool := board.get pos == Cell.Empty
 
 def switchPlayer (player : Player) : Player :=
   match player with
   | Player.X => Player.O
   | Player.O => Player.X
+
+theorem switchPlayerIdentity (player : Player) : switchPlayer (switchPlayer player) = player := by
+  simp [switchPlayer]
+  match player with
+  | Player.X => trivial
+  | Player.O => trivial
+
+theorem switchPlayerNeg (player : Player) : ¬switchPlayer player = player := by
+  simp [switchPlayer]
+  match player with
+  | Player.X => trivial
+  | Player.O => trivial
 
 def isBoardFull (board : Board) : Bool :=
   (List.finRange 9).all (fun i =>
@@ -55,9 +144,10 @@ def checkWin (board : Board) (player : Player) : Bool :=
     -- Diagonals
     [0, 4, 8], [2, 4, 6]
   ]
+
+  -- We use ≥ here to make our proofs easier
   winningLines.any (fun line =>
-    line.all (fun pos =>
-      board.get pos == playerCell))
+    line.countP (fun pos => board.get pos == playerCell) >= 3)
 
 def wellFormedGame (state : TicTacToeState) : Bool :=
   match state.status with
@@ -65,10 +155,8 @@ def wellFormedGame (state : TicTacToeState) : Bool :=
       !isBoardFull state.board
       && !checkWin state.board Player.X
       && !checkWin state.board Player.O
-  | GameStatus.Won Player.X =>
-      checkWin state.board Player.X && !checkWin state.board Player.O
-  | GameStatus.Won Player.O =>
-      !checkWin state.board Player.X && checkWin state.board Player.O
+  | GameStatus.Won player =>
+      checkWin state.board player && !checkWin state.board (switchPlayer player)
   | GameStatus.Draw =>
       isBoardFull state.board
       && !checkWin state.board Player.X
@@ -104,7 +192,7 @@ theorem initialGameStateIsWellFormed (state : TicTacToeState) {h: state = initia
 
   simp [hCheckWinEmpty Player.X, hCheckWinEmpty Player.O, hBoardNotFull]
 
-def makeMove {player : Player} (state : TicTacToeState) (pos : Position) (_ : state.status = GameStatus.InProgress player) (_ : isEmptyPosition state.board pos) : TicTacToeState :=
+def makeMove {player : Player} (state : TicTacToeState) (pos : Position) (_ : state.status = GameStatus.InProgress player) (_ : isEmptyPosition state.board pos) (_ : wellFormedGame state) : TicTacToeState :=
   let newBoard := state.board.set pos.val (Cell.Occupied player)
   let newStatus :=
     if checkWin newBoard player then
@@ -115,6 +203,145 @@ def makeMove {player : Player} (state : TicTacToeState) (pos : Position) (_ : st
       GameStatus.InProgress (switchPlayer player)
   { board := newBoard, status := newStatus }
 
+theorem noWinWithoutOwnMove
+  (board : Board) (player : Player) (pos : Position) (hIsEmpty : isEmptyPosition board pos) (hNoWin : checkWin board player = false)
+  : checkWin (Vector.set board pos.val (Cell.Occupied (switchPlayer player))) player = false := by
+
+  -- `newBoard` is the board after the other player has made a move
+  let newBoard := Vector.set board pos.val (Cell.Occupied (switchPlayer player))
+
+  -- The cell at pos is now occupied by them
+  have cellAtPosIsOccupiedByOtherPlayer : Vector.get newBoard pos = Cell.Occupied (switchPlayer player) := by
+    simp [isEmptyPosition] at hIsEmpty
+    match hMatch : Vector.get board pos with
+    | Cell.Occupied a => simp [hMatch] at hIsEmpty
+    | Cell.Empty => simp [newBoard, Vector.set, Vector.get]
+
+  -- Other cells were not modified
+  have getFromNewBoardRespectsPreviouslyOccupied {i} {hIsNotPos : ¬pos = i}
+    : Vector.get newBoard i = Vector.get board i := by
+    simp at hIsNotPos
+    let hGetFromBoardUnchanged := vectorSetGetUnchanged (xs := board) (value := Cell.Occupied (switchPlayer player)) (hDistinct := hIsNotPos)
+    simp [newBoard, hGetFromBoardUnchanged]
+
+  simp [checkWin] at hNoWin
+  simp [checkWin]
+
+  have setAnywhereLeavesSelectionUntouched {i}
+    : (Vector.get board i == Cell.Occupied player) = (Vector.get newBoard i == Cell.Occupied player) := by
+    by_cases hPos : pos = i
+    .
+      simp [isEmptyPosition] at hIsEmpty
+      simp [← hPos, cellAtPosIsOccupiedByOtherPlayer, hIsEmpty, cellNeqEmptyOccupied, switchPlayerNeg]
+    .
+      let hGetFromBoardUnchanged := getFromNewBoardRespectsPreviouslyOccupied (hIsNotPos := hPos)
+      exact Eq.symm (congrArg (· == Cell.Occupied player) hGetFromBoardUnchanged)
+
+  -- For each count, we know that it doesn't change after the Vector.set
+  have noCountChange
+    {x y z : Position}
+    (hCountBeforeMove : List.countP (fun i => Vector.get board i == Cell.Occupied player) [x, y, z] < 3)
+    : List.countP (fun i => Vector.get newBoard i == Cell.Occupied player) [x, y, z] < 3 := by
+
+    -- Unfold
+    simp [List.countP, List.countP.go, List.countP.go, List.countP.go]
+
+    -- Rewrite
+    simp [
+      (setAnywhereLeavesSelectionUntouched (i := x)).symm,
+      (setAnywhereLeavesSelectionUntouched (i := y)).symm,
+      (setAnywhereLeavesSelectionUntouched (i := z)).symm,
+    ]
+
+    -- Fold back
+    change List.countP (fun i => Vector.get board i == Cell.Occupied player) [x, y, z] < 3
+    exact hCountBeforeMove
+
+  simp [
+    newBoard,
+    noCountChange hNoWin.left,
+    noCountChange hNoWin.right.left,
+    noCountChange hNoWin.right.right.left,
+    noCountChange hNoWin.right.right.right.left,
+    noCountChange hNoWin.right.right.right.right.left,
+    noCountChange hNoWin.right.right.right.right.right.left,
+    noCountChange hNoWin.right.right.right.right.right.right.left,
+    noCountChange hNoWin.right.right.right.right.right.right.right,
+  ]
+
+theorem makeMovePreservesWellFormedness
+  {state : TicTacToeState}
+  {currentPlayer : Player}
+  {pos : Position}
+  {hInProgress : state.status = GameStatus.InProgress currentPlayer}
+  {hIsEmpty : isEmptyPosition state.board pos}
+  {hWellFormed : wellFormedGame state}
+  : wellFormedGame (makeMove state pos hInProgress hIsEmpty hWellFormed) := by
+  let newState := (makeMove state pos hInProgress hIsEmpty hWellFormed)
+  let newBoard := newState.board
+  have hNewBoard : newBoard = Vector.set state.board pos.val (Cell.Occupied currentPlayer) := by
+    trivial
+
+  have hNoWinnersYet : checkWin state.board currentPlayer = false ∧ checkWin state.board (switchPlayer currentPlayer) = false := by
+    unfold wellFormedGame at hWellFormed
+    simp [hInProgress] at hWellFormed
+    match currentPlayer with
+    | Player.X => simp [switchPlayer, hWellFormed]
+    | Player.O => simp [switchPlayer, hWellFormed]
+
+  simp [wellFormedGame, hInProgress] at hWellFormed
+  simp [makeMove]
+
+  match hMatch : (checkWin newBoard currentPlayer, checkWin newBoard (switchPlayer currentPlayer)) with
+  | (true, false) =>
+    -- We have a winner!
+    let hWonLeft := congrArg (fun x => x.1) hMatch
+    simp at hWonLeft
+    let hWonRight := congrArg (fun x => x.2) hMatch
+    simp at hWonRight
+    simp [wellFormedGame, ← hNewBoard, hWonLeft, hWonRight]
+  | (false, false) =>
+    let hWonLeft := congrArg (fun x => x.1) hMatch
+    simp at hWonLeft
+    let hWonRight := congrArg (fun x => x.2) hMatch
+    simp at hWonRight
+    simp [wellFormedGame, ← hNewBoard, hWonLeft]
+    by_cases hDraw : isBoardFull newBoard
+    . -- Draw
+      simp [hDraw]
+      match hCurrentPlayer : currentPlayer with
+      | Player.X =>
+        simp [hCurrentPlayer] at hWonLeft
+        simp [switchPlayer, hCurrentPlayer] at hWonRight
+        simp [hWonLeft, hWonRight]
+      | Player.O =>
+        simp [hCurrentPlayer] at hWonLeft
+        simp [switchPlayer, hCurrentPlayer] at hWonRight
+        simp [hWonLeft, hWonRight]
+    . -- The game goes on
+      simp [hDraw]
+      match hCurrentPlayer : currentPlayer with
+      | Player.X =>
+        simp [hCurrentPlayer] at hWonLeft
+        simp [switchPlayer, hCurrentPlayer] at hWonRight
+        simp [hWonLeft, hWonRight]
+      | Player.O =>
+        simp [hCurrentPlayer] at hWonLeft
+        simp [switchPlayer, hCurrentPlayer] at hWonRight
+        simp [hWonLeft, hWonRight]
+  | (_, true) =>
+    -- This branch is unreachable, so the known facts at this point must lead to a contradiction.
+    let hWonLeft := congrArg (fun x => x.1) hMatch
+    simp at hWonLeft
+    let hWonRight := congrArg (fun x => x.2) hMatch
+    simp at hWonRight
+
+    -- If the other player already won, it must have won before the last move, which
+    -- is impossible (it would mean the game state was not well formed at the last move)
+    let hNoPreviousWinner := noWinWithoutOwnMove state.board (switchPlayer currentPlayer) pos hIsEmpty hNoWinnersYet.right
+    simp [switchPlayerIdentity, ← hNewBoard] at hNoPreviousWinner
+    simp [hNoPreviousWinner] at hWonRight
+
 -- Proof: players alternate after each move
 theorem playersAlternateAfterMove
   {state : TicTacToeState}
@@ -122,9 +349,10 @@ theorem playersAlternateAfterMove
   {pos : Position}
   {hInProgress : state.status = GameStatus.InProgress currentPlayer}
   {hIsEmpty : isEmptyPosition state.board pos}
+  {hWellFormed : wellFormedGame state}
   {newState : TicTacToeState}
   (
-    h: makeMove state pos hInProgress hIsEmpty = newState
+    h: makeMove state pos hInProgress hIsEmpty hWellFormed = newState
   ) : (
     newState.status = GameStatus.InProgress (switchPlayer currentPlayer) ∨
     newState.status = GameStatus.Won currentPlayer ∨
@@ -134,7 +362,7 @@ theorem playersAlternateAfterMove
   simp at h'
   rw [Eq.symm h']
 
-  match hMatch : (makeMove state pos hInProgress hIsEmpty).status with
+  match hMatch : (makeMove state pos hInProgress hIsEmpty hWellFormed).status with
   | GameStatus.Won winner =>
     -- Get ourselves a clear goal
     right
@@ -168,9 +396,10 @@ theorem cellMarkedAfterMove
   {pos : Position}
   {hInProgress : state.status = GameStatus.InProgress currentPlayer}
   {hIsEmpty : isEmptyPosition state.board pos}
+  {hWellFormed : wellFormedGame state}
   {newState : TicTacToeState}
   (
-    h: makeMove state pos hInProgress hIsEmpty = newState
+    h: makeMove state pos hInProgress hIsEmpty hWellFormed = newState
   ) : (
     newState.board.get pos = Cell.Occupied currentPlayer
   ) := by
